\[
H=\frac{p_{r}^{2}}{2 m}+\frac{p_{\theta}^{2}}{2 m r^{2}}+V(r)
\]
Write $W=W_{r}+W_{\theta} ;$ then the time-independent HJ equation is
\[
\frac{1}{2 m}\left[\left(\frac{\partial W_{r}}{\partial r}\right)^{2}+\frac{1}{r^{2}}\left(\frac{\partial W_{\theta}}{\partial \theta}\right)^{2}\right]+V(r)=Q_{1} \equiv E
\]
(we use subscripts on the $Q$ s so as not to confuse the indices with powers). This is where the procedure of ( 6.14) comes in. If both sides are multiplied by $f(r)=2 m r^{2}$ this equation becomes
\[
r^{2}\left(\frac{\partial W_{r}}{\partial r}\right)^{2}+2 m r^{2} V(r)-2 m r^{2} Q_{1}=-\left(\frac{\partial W_{\theta}}{\partial \theta}\right)^{2}
\]
which separates the $r$ and $\theta$ parts. Thus
\[
\begin{array}{l}
{W_{r}^{\prime}=\sqrt{2 m Q_{1}-2 m V(r)-r^{-2} Q_{2}^{2}}} \\
{W_{\theta}^{\prime}=Q_{2}}
\end{array}
\]
Integration then yields
$\left.\begin{array}{rl}{W_{r}(r)} & {=\sqrt{2 m} \int \sqrt{Q_{1}-V(r)-\left(2 m r^{2}\right)^{-1} Q_{2}^{2}} d r,} \\ {W_{\theta}(\theta)} & {=Q_{2} \theta}\end{array}\right\}$
